organize, add implementation of H', add hypothesis about same results in commutative region

definitions.v
@@ -12,197 +12,243 @@ Import ListNotations.
 Require Import OrderedType.
 Require Import Ensembles.
 
-Definition tid : Type := nat.
-Definition all_tid := 0. (* XXX probably needs to change *)
-Inductive action : Type :=
+Section State.
+
+  Definition tid : Type := nat.
+  Definition all_tid := 0. (* XXX probably needs to change *)
+
+  Definition thread_history_state : Type := tid -> nat.
+  Definition thread_commute_state : Type := tid -> nat. (* 0 or 1 *)
+  Definition refstate : Type := nat.
+  Inductive state := State : refstate -> thread_history_state -> thread_commute_state -> state.
+
+End State.
+
+Section Histories.
+
+  Inductive action : Type :=
 | ActInv (tid : tid) : action
 | ActResp (tid : tid) : action
 | Continue (tid: tid) : action
 | Emulate (tid: tid) : action
 | Commute (tid: tid) : action.
-Definition history : Type := list action.
 
-(* where the start of the commutative region of history begins *)
-Parameter commute_index : nat. 
-Definition thread_history_state : Type := tid -> nat.
-Definition thread_commute_state : Type := tid -> nat. (* 0 or 1 *)
-Definition refstate : Type := nat.
-Inductive state := State : refstate -> thread_history_state -> thread_commute_state -> state.
+  Definition thread_of_action (a: action) :=
+    match a with 
+      | ActInv t | ActResp t | Continue t
+      | Emulate t | Commute t => t
+    end.
+  Definition action_eq (a1 a2: action) :=
+    match a1, a2 with
+      | Commute t, Commute t'
+      | Emulate t, Emulate t'
+      | ActInv t, ActInv t'
+      | ActResp t, ActResp t'
+      | Continue t, Continue t' => t =? t'
+      | _, _ => false
+    end.
+  Definition history : Type := list action.
 
-Inductive event : Type := Event (t: tid) (s1 s2 : state) (a r : action) : event.
-Definition trace : Type := list event.
-Function history_of_trace (tr: trace) : history :=
-  match tr with
-  | [] => []
-  | Event t s1 s2 a r :: tl =>
-    match a,r with
-             | Continue t, Continue t' => history_of_trace tl
-             | Continue t, _ => r :: history_of_trace tl
-             | _, Continue t => a :: history_of_trace tl
-             | _,_ => a :: r :: history_of_trace tl
-             end
-  end.
+  Inductive event : Type := Event (t: tid) (s1 s2 : state) (a r : action) : event.
+  Definition trace : Type := list event.
+  Function history_of_trace (tr: trace) : history :=
+    match tr with
+      | [] => []
+      | Event t s1 s2 a r :: tl =>
+        match a,r with
+          | Continue t, Continue t' => history_of_trace tl
+          | Continue t, _ => r :: history_of_trace tl
+          | _, Continue t => a :: history_of_trace tl
+          | _,_ => a :: r :: history_of_trace tl
+        end
+    end.
+  Function invocations_of_trace (tr:trace) : list action :=
+    filter (fun a => match a with | ActInv _ => true | _ => false end) (history_of_trace tr).
     
-Definition swappable (a1 a2 : action) :=
-  match a1, a2 with
-  | ActInv t, ActInv t'
-  | ActInv t, ActResp t'
-  | ActResp t, ActInv t'
-  | ActResp t, ActResp t' => t <> t'
-  | _, _ => False
-  end.
-Inductive reordered : relation history :=
-| ro_perm_nil : reordered [] []
-| ro_perm_skip : forall x t1 t2,
-    reordered t1 t2 ->
-    reordered (x::t1) (x::t2)
-| ro_perm_swap : forall a2 a1 t,
-    swappable a2 a1 ->
-    reordered (a2 :: a1 :: t) (a1 :: a2 :: t)
-| ro_perm_trans : forall t1 t2 t3,
-    reordered t1 t2 ->
-    reordered t2 t3 ->
-    reordered t1 t3.
+  Definition swappable (a1 a2 : action) :=
+    match a1, a2 with
+      | ActInv t, ActInv t'
+      | ActInv t, ActResp t'
+      | ActResp t, ActInv t'
+      | ActResp t, ActResp t' => t <> t'
+      | _, _ => False
+    end.
+  Inductive reordered : relation history :=
+  | ro_perm_nil : reordered [] []
+  | ro_perm_skip : forall x t1 t2,
+                     reordered t1 t2 ->
+                     reordered (x::t1) (x::t2)
+  | ro_perm_swap : forall a2 a1 t,
+                     swappable a2 a1 ->
+                     reordered (a2 :: a1 :: t) (a1 :: a2 :: t)
+  | ro_perm_trans : forall t1 t2 t3,
+                      reordered t1 t2 ->
+                      reordered t2 t3 ->
+                      reordered t1 t3.
 
-Definition write_tid_set (ts1 ts2 : tid -> nat) : Ensemble tid :=
-  fun tid => ts1 tid <> ts2 tid.
-Definition step_writes (s1 s2 : state) : Ensemble tid :=
-  match s1, s2 with
-  | State rs1 th1 tc1, State rs2 th2 tc2 =>
-    let writes_tid := Union tid (write_tid_set th1 th2) (write_tid_set tc1 tc2) in
-    if rs1 =? rs2 then writes_tid
-    else Add tid writes_tid all_tid
-  end.
-Function trace_writes (tr : trace) : Ensemble tid :=
-  match tr with
-  | [] => Empty_set tid
-  | Event t s1 s2 a r :: tl =>
-    Union tid (step_writes s1 s2) (trace_writes tl)
-  end.
-Function trace_conflict_free (tr : trace) : Prop :=
-  match tr with
-  | [] => False
-  | Event t s1 s2 a r :: tl =>
-    Intersection tid (step_writes s1 s2) (trace_writes tl) = Empty_set tid
-    /\ trace_conflict_free tl
-  end.
-                                                                          
-Definition sim_commutes (h : history) : Prop. Admitted.
+End Histories.
 
-Parameter ref_impl : (refstate * action) -> (refstate * action).
-Parameter spec : list history.
+Section Commutativity.
+  Definition write_tid_set (ts1 ts2 : tid -> nat) : Ensemble tid :=
+    fun tid => ts1 tid <> ts2 tid.
+  Definition step_writes (s1 s2 : state) : Ensemble tid :=
+    match s1, s2 with
+      | State rs1 th1 tc1, State rs2 th2 tc2 =>
+        let writes_tid := Union tid (write_tid_set th1 th2) (write_tid_set tc1 tc2) in
+        if rs1 =? rs2 then writes_tid
+        else Add tid writes_tid all_tid
+    end.
+  Function trace_writes (tr : trace) : Ensemble tid :=
+    match tr with
+      | [] => Empty_set tid
+      | Event t s1 s2 a r :: tl =>
+        Union tid (step_writes s1 s2) (trace_writes tl)
+    end.
+  Function trace_conflict_free (tr : trace) : Prop :=
+    match tr with
+      | [] => False
+      | Event t s1 s2 a r :: tl =>
+        Intersection tid (step_writes s1 s2) (trace_writes tl) = Empty_set tid
+        /\ trace_conflict_free tl
+    end.
 
-Inductive ref_impl_generated_trace : trace -> state -> state -> Prop :=
-| RINil : forall s, ref_impl_generated_trace [] s s
-| RICons : forall rs a rs' r tr rs0 th tc, 
-    ref_impl (rs, a) = (rs', r) ->
-    ref_impl_generated_trace tr (State rs0 th tc) (State rs th tc) ->
-    ref_impl_generated_trace ((Event all_tid (State rs th tc) (State rs' th tc) a r) :: tr)
-                             (State rs0 th tc) (State rs' th tc).
-Hypothesis ref_impl_correct : forall (tr : trace) (s1 s2 : state),
-    ref_impl_generated_trace tr s1 s2 ->
-    List.In (history_of_trace tr) spec.
-Hypothesis SIM_reordered_histories_correct : forall tr0 tr1 tr2 tr1' : trace,
-    List.In (history_of_trace (tr0 ++ tr1 ++ tr2)) spec ->
-    sim_commutes (history_of_trace tr1) ->
-    reordered (history_of_trace tr1) (history_of_trace tr1') ->
-    List.In (history_of_trace (tr0 ++ tr1' ++ tr2)) spec.
+  Definition sim_commutes (h : history) : Prop. Admitted.
+End Commutativity.
 
-Definition thread_of_action (a: action) :=
-  match a with 
-  | ActInv t | ActResp t | Continue t
-  | Emulate t | Commute t => t
-  end.
-Definition action_eq (a1 a2: action) :=
-  match a1, a2 with
-  | Commute t, Commute t'
-  | Emulate t, Emulate t'
-  | ActInv t, ActInv t'
-  | ActResp t, ActResp t'
-  | Continue t, Continue t' => t =? t'
-  | _, _ => false
-  end.
+Section Emulator.
+  Parameter ref_impl : (refstate * action) -> (refstate * action).
+  Parameter spec : list history.
+  Parameter num_threads : nat.
+  Hypothesis tid_le_num_threads : forall tid, tid <= num_threads.
 
-Definition inc_index (th : tid -> nat) (t: tid) :=
-  fun tid => if tid =? t then th tid + 1 else th tid.
-Definition set_index (tc : tid -> nat) (t : tid) :=
-  fun tid => if tid =? t then 1 else tc t.
-Definition try_enter_conflict_free_mode (hbase: history) (s: state) (t: tid) : state :=
-  match s with
-  | State rs th tc =>
-    let hd := nth (th t) hbase (Emulate t) in
-    let tc' := if action_eq hd (Commute t) then set_index tc t else tc in
-    let th' := if action_eq hd (Commute t) then inc_index th t else th in
-    State rs th' tc'
-  end.
-Definition try_switch_to_emulate (hbase : history) (s : state) (a : action) (t : tid) : state :=
-  match s with
-  | State rs th tc =>
-    let hd := nth (th t) hbase (Emulate t) in
-    if  eqb (action_eq hd a) false
-            && (eqb (action_eq a (Continue t)) false || eqb (action_eq hd (ActResp t)) false)
-            && eqb (action_eq hd (Emulate t)) false
-    then let th' := fun tid => (length hbase) + 1 in (* always return Emulate *)
-         let rs' := rs in(* TODO process H' or something*)
-         State rs' th' tc
-    else s
-  end.
-Definition emulator_act
-           (hbase : history) (s : state) (a : action) : (state * action) :=
-  let t := thread_of_action a in
-  let s' := try_enter_conflict_free_mode hbase s t in
-  let s'' := try_switch_to_emulate hbase s' a t in
-  match s'' with
-  | State rs th tc => 
-    let hd := nth (th t) hbase (Emulate t) in
-    let (rs', r) := if action_eq hd a then (rs, Continue t)
-                    else if action_eq a (Continue t) && action_eq hd (ActResp t)
-                         then (rs, hd)
-                         else ref_impl (rs, a) in (* XXX we know we must be in emulate mode *)
-    if action_eq hd (Emulate t) then (State rs' th tc, r) (* emulate mode *)
-    else let th' := if tc t =? 1 then inc_index th t (* conflict-free mode *)
-                    else fun tid => (th tid) + 1 in (* replay mode *)
-         (State rs th' tc, r)
-  end.
-Function emulator_trace (hbase hrun : history) (s0 : state) (tr : trace) : trace :=
-  match hrun with
-  | [] => tr
-  | a :: rest => let (s', r) := emulator_act hbase s0 a in
-                 let t := thread_of_action a in
-                 emulator_trace hbase rest s' (Event t s0 s' a r :: tr)
-  end.
+  Inductive ref_impl_generated_trace : trace -> state -> state -> Prop :=
+  | RINil : forall s, ref_impl_generated_trace [] s s
+  | RICons : forall rs a rs' r tr rs0 th tc, 
+               ref_impl (rs, a) = (rs', r) ->
+               ref_impl_generated_trace tr (State rs0 th tc) (State rs th tc) ->
+               ref_impl_generated_trace ((Event all_tid (State rs th tc) (State rs' th tc) a r) :: tr)
+                                        (State rs0 th tc) (State rs' th tc).
+  Hypothesis ref_impl_correct : forall (tr : trace) (s1 s2 : state),
+                                  ref_impl_generated_trace tr s1 s2 ->
+                                  List.In (history_of_trace tr) spec.
 
-(* if we have a correct trace whose corresponding history is SIM-comm,
- * then the emulator produces a conflict-free trace for that history *)
-Lemma emulator_impl_conflict_free : forall t tr s0 s1,
-    ref_impl_generated_trace tr s0 s1 ->
-    sim_commutes (history_of_trace tr) ->
-    trace_conflict_free (emulator_trace (Commute t :: (history_of_trace tr))
-                                        (history_of_trace tr)
-                                        s0 []).
-Proof.
-Admitted.
+  Hypothesis comm_region_ref_impl_produces_same_results : 
+    forall tr tr' s0 sf sf', sim_commutes (history_of_trace tr) ->
+                             ref_impl_generated_trace tr s0 sf ->
+                             ref_impl_generated_trace tr' s0 sf' ->
+                             invocations_of_trace tr = invocations_of_trace tr' ->
+                             reordered (history_of_trace tr') (history_of_trace tr).
+              
+  Hypothesis SIM_reordered_histories_correct :
+    forall tr0 tr1 tr2 tr1' : trace,
+      List.In (history_of_trace (tr0 ++ tr1 ++ tr2)) spec ->
+      sim_commutes (history_of_trace tr1) ->
+      reordered (history_of_trace tr1) (history_of_trace tr1') ->
+      List.In (history_of_trace (tr0 ++ tr1' ++ tr2)) spec.
+  
+  Definition inc_index (th : tid -> nat) (t: tid) :=
+    fun tid => if tid =? t then th tid + 1 else th tid.
+  Definition set_index (tc : tid -> nat) (t : tid) :=
+    fun tid => if tid =? t then 1 else tc t.
+  Definition try_enter_conflict_free_mode (hbase: history) (s: state) (t: tid) : state :=
+    match s with
+      | State rs th tc =>
+        let hd := nth (th t) hbase (Emulate t) in
+        let tc' := if action_eq hd (Commute t) then set_index tc t else tc in
+        let th' := if action_eq hd (Commute t) then inc_index th t else th in
+        State rs th' tc'
+    end.
+  Function ref_impl_replay_helper (hbase : history)
+           (th: tid -> nat) (t: tid) (rs : refstate)
+  : refstate :=    
+    match t with
+      | 0 => rs
+      | S t' => let new_rs := fold_left
+                                (fun rs a => let (rs', r) :=
+                                                 match a with
+                                                   | ActInv _ => ref_impl (rs, a)
+                                                   | _ => (rs, a) end
+                                             in rs')
+                                       (firstn (th t) hbase) rs
+               in ref_impl_replay_helper hbase th t' new_rs
+    end.
+  Definition ref_impl_replay (hbase: history) (th: tid -> nat) (rs0 : refstate) : refstate :=
+    ref_impl_replay_helper hbase th num_threads rs0.
+  Definition try_switch_to_emulate (hbase : history) (s : state) (a : action) (t : tid) : state :=
+    match s with
+      | State rs th tc =>
+        let hd := nth (th t) hbase (Emulate t) in
+        if eqb (action_eq hd a) false
+                && (eqb (action_eq a (Continue t)) false || eqb (action_eq hd (ActResp t)) false)
+                && eqb (action_eq hd (Emulate t)) false
+        then let th' := fun tid => (length hbase) + 1 in (* always return Emulate *)
+             let rs' := ref_impl_replay hbase th rs in
+             State rs' th' tc
+        else s
+    end.
+  Definition emulator_act
+             (hbase : history) (s : state) (a : action) : (state * action) :=
+    let t := thread_of_action a in
+    let s' := try_enter_conflict_free_mode hbase s t in
+    let s'' := try_switch_to_emulate hbase s' a t in
+    match s'' with
+      | State rs th tc => 
+        let hd := nth (th t) hbase (Emulate t) in
+        let (rs', r) := if action_eq hd a then (rs, Continue t)
+                        else if action_eq a (Continue t) && action_eq hd (ActResp t)
+                             then (rs, hd)
+                             else ref_impl (rs, a) in (* XXX we know we must be in emulate mode *)
+        if action_eq hd (Emulate t) then (State rs' th tc, r) (* emulate mode *)
+        else let th' := if tc t =? 1 then inc_index th t (* conflict-free mode *)
+                        else fun tid => (th tid) + 1 in (* replay mode *)
+             (State rs th' tc, r)
+    end.
+  Function emulator_trace (hbase hrun : history) (s0 : state) (tr : trace) : trace :=
+    match hrun with
+      | [] => tr
+      | a :: rest => let (s', r) := emulator_act hbase s0 a in
+                     let t := thread_of_action a in
+                     emulator_trace hbase rest s' (Event t s0 s' a r :: tr)
+    end.
 
-(* if we have the emulator instantiated with a SIM-comm history,
- * and the emulator acts on some input sequence, then the emulator
- * produces a correct trace for the spec *)
-Lemma emulator_impl_correct : forall t tr s0 s1 h,
-    ref_impl_generated_trace tr s0 s1 ->
-    sim_commutes (history_of_trace tr) ->
-    List.In (history_of_trace (emulator_trace (Commute t :: history_of_trace tr)
-                                              h s0 []))
-            spec.
-Proof.
-Admitted.
+End Emulator.
 
-Theorem scalable_commutativity_rule : forall t tr s0 s1 h,
-    ref_impl_generated_trace tr s0 s1 ->
-    sim_commutes (history_of_trace tr) ->
-    trace_conflict_free (emulator_trace (Commute t :: (history_of_trace tr))
-                                        (history_of_trace tr) s0 [])
-    /\ List.In
-         (history_of_trace (emulator_trace (Commute t :: history_of_trace tr) h s0 []))
-         spec.
-Proof.
-  intros; split; [eapply emulator_impl_conflict_free | eapply emulator_impl_correct]; eauto.
-Qed.
+Section Theorems.
+  (* if we have a correct trace whose corresponding history is SIM-comm,
+   * then the emulator produces a conflict-free trace for that history *)
+  Lemma emulator_impl_conflict_free :
+    forall t tr s0 s1,
+      ref_impl_generated_trace tr s0 s1 ->
+      sim_commutes (history_of_trace tr) ->
+      trace_conflict_free (emulator_trace (Commute t :: (history_of_trace tr))
+                                          (history_of_trace tr)
+                                          s0 []).
+  Proof.
+  Admitted.
+
+  (* if we have the emulator instantiated with a SIM-comm history,
+   * and the emulator acts on some input sequence, then the emulator
+   * produces a correct trace for the spec *)
+  Lemma emulator_impl_correct :
+    forall t tr s0 s1 h,
+      ref_impl_generated_trace tr s0 s1 ->
+      sim_commutes (history_of_trace tr) ->
+      List.In (history_of_trace (emulator_trace (Commute t :: history_of_trace tr)
+                                                h s0 []))
+              spec.
+  Proof.
+  Admitted.
+
+  Theorem scalable_commutativity_rule :
+    forall t tr s0 s1 h,
+      ref_impl_generated_trace tr s0 s1 ->
+      sim_commutes (history_of_trace tr) ->
+      trace_conflict_free (emulator_trace (Commute t :: (history_of_trace tr))
+                                          (history_of_trace tr) s0 [])
+      /\ List.In
+           (history_of_trace (emulator_trace (Commute t :: history_of_trace tr) h s0 []))
+           spec.
+  Proof.
+    intros; split; [eapply emulator_impl_conflict_free | eapply emulator_impl_correct]; eauto.
+  Qed.
+End Theorems.
